fairness/fairness_finiteness.v
@@ -28,21 +28,60 @@ Section finitary.
 
   Context `{HPI0: forall s x, ProofIrrel ((let '(s', ℓ) := x in M.(fmtrans) s ℓ s'): Prop) }.
 
-  Variable model_finitary: forall s1, Finite { '(s2, ℓ) | M.(fmtrans) s1 ℓ s2 }.
+  Variable (ξ: execution_trace Λ -> finite_trace M (option M.(fmrole)) -> Prop).
 
-  Definition enum_inner (s1: M): list (M * option M.(fmrole)) :=
-    map proj1_sig (@enum _ _ (model_finitary s1)).
+  Variable model_finitary: rel_finitary ξ.
 
-  Lemma enum_inner_spec (s1 s2: M) ℓ:
-    M.(fmtrans) s1 ℓ s2 -> (s2, ℓ) ∈ enum_inner s1.
+  #[local] Instance eq_dec_next_states ex atr c' oζ:
+    EqDecision {'(δ', ℓ) : M * (option (fmrole M)) |
+                  ξ (ex :tr[ oζ ]: c') (atr :tr[ ℓ ]: δ')}.
+  Proof. intros x y. apply make_decision. Qed.
+
+  Lemma model_finite: ∀ (ex : execution_trace Λ) (atr : finite_trace _ _) c' oζ,
+    Finite (sig (λ '(δ', ℓ), ξ (ex :tr[oζ]: c') (atr :tr[ℓ]: δ'))).
   Proof.
-    intros H. unfold enum_inner. rewrite elem_of_list_fmap.
-    exists (exist _ (s2, ℓ) H). split =>//. apply elem_of_enum.
+    intros ex atr c' oζ.
+    pose proof (model_finitary ex atr c' oζ).
+    by apply smaller_card_nat_finite in H.
   Qed.
 
-  Program Definition enumerate_next (δ1: LM) (oζ : olocale Λ) (c': cfg Λ):
+  Definition enum_inner extr fmodtr c' oζ : list (M * option M.(fmrole)) :=
+    map proj1_sig (@enum _ _ (model_finite extr fmodtr c' oζ)).
+
+  Lemma enum_inner_spec (δ' : M) ℓ extr atr c' oζ :
+    ξ (extr :tr[oζ]: c') (atr :tr[ℓ]: δ') → (δ', ℓ) ∈ enum_inner extr atr c' oζ.
+  Proof.
+    intros H. unfold enum_inner. rewrite elem_of_list_fmap.
+    exists (exist _ (δ', ℓ) H). split =>//. apply elem_of_enum.
+  Qed.
+
+  (* TODO: move *)
+  Fixpoint trace_map {A A' L L'} (sf: A → A') (lf: L -> L') (tr: finite_trace A L): finite_trace A' L' :=
+  match tr with
+  | trace_singleton x => trace_singleton $ sf x
+  | trace_extend tr' ℓ x => trace_extend (trace_map sf lf tr') (lf ℓ) (sf x)
+  end.
+
+  Fixpoint get_underlying_fairness_trace (M : FairModel) (LM: LiveModel Λ M) (ex : auxiliary_trace LM) :=
+  match ex with
+  | trace_singleton δ => trace_singleton (ls_under δ)
+  | trace_extend ex' (Take_step ρ _) δ => trace_extend (get_underlying_fairness_trace M LM ex') ρ (ls_under δ)
+  | trace_extend ex' _ _ => get_underlying_fairness_trace M LM ex'
+  end.
+
+  Definition get_role {M : FairModel} {LM: LiveModel Λ M} (lab: mlabel LM) :=
+  match lab with
+  | Take_step ρ _ => Some ρ
+  | _ => None
+  end.
+
+  Definition map_underlying_trace {M : FairModel} {LM: LiveModel Λ M} (aux : auxiliary_trace LM) :=
+    (trace_map (λ s, ls_under s) (λ lab, get_role lab) aux).
+
+  Program Definition enumerate_next extr (fmodtr: auxiliary_trace LM) c' oζ:
     list (LM * @mlabel LM) :=
-    '(s2, ℓ) ← (δ1.(ls_under), None) :: enum_inner δ1.(ls_under);
+    let δ1 := trace_last fmodtr in
+    '(s2, ℓ) ← (δ1.(ls_under), None) :: enum_inner extr (map_underlying_trace fmodtr) c' oζ;
     d ← enumerate_dom_gsets' (dom δ1.(ls_fuel) ∪ live_roles _ s2);
     fs ← enum_gmap_bounded' (live_roles _ s2 ∪ d) (max_gmap δ1.(ls_fuel) `max` LM.(fuel_limit) s2);
     ms ← enum_gmap_range_bounded' (live_roles _ s2 ∪ d) (locales_of_list c'.1);
@@ -70,19 +109,153 @@ Section finitary.
   Qed.
 
   Lemma valid_state_evolution_finitary_fairness (φ: execution_trace Λ -> auxiliary_trace LM -> Prop) :
+    rel_finitary (valid_lift_fairness (λ extr auxtr, ξ extr (map_underlying_trace auxtr) ∧ φ extr auxtr)).
+  Proof.
+    rewrite /valid_lift_fairness.
+    intros ex atr [e' σ'] oζ.
+    eapply finite_smaller_card_nat.
+    simpl.
+    eapply (in_list_finite (enumerate_next ex atr (e',σ') oζ)).
+    intros [δ' ℓ] [[Hlbl [Htrans Htids]] [Hξ Hφ]].
+    unfold enumerate_next. apply elem_of_list_bind.
+    exists (δ'.(ls_under), match ℓ with Take_step l _ => Some l | _ => None end).
+    split; last first.
+    { destruct ℓ as [ρ tid' | |].
+      - inversion Htrans as [Htrans']. apply elem_of_cons; right.
+        by apply enum_inner_spec.
+      - apply elem_of_cons; left. f_equal. inversion Htrans as (?&?&?&?&?); done.
+      - apply elem_of_cons; right. inversion Htrans as (?&?). by apply enum_inner_spec. }
+    apply elem_of_list_bind. eexists (dom $ δ'.(ls_fuel)). split; last first.
+    { apply enumerate_dom_gsets'_spec. destruct ℓ as [ρ tid' | |].
+      - inversion Htrans as (?&?&?&?&?&?&?). intros ρ' Hin. destruct (decide (ρ' ∈ live_roles _ δ')); first set_solver.
+        destruct (decide (ρ' ∈ dom $ ls_fuel (trace_last atr))); first set_solver. set_solver.
+      - inversion Htrans as (?&?&?&?&?). set_solver.
+      - inversion Htrans as (?&?&?&?&?). done. }
+    apply elem_of_list_bind.
+    assert (Hfueldom: dom δ'.(ls_fuel) = live_roles M δ' ∪ dom (ls_fuel δ')).
+    { rewrite subseteq_union_1_L //. apply ls_fuel_dom. }
+    eexists (δ'.(ls_fuel) ↾ Hfueldom); split; last first.
+    { eapply enum_gmap_bounded'_spec; split =>//.
+      intros ρ f Hsome. destruct ℓ as [ρ' tid' | |].
+      - destruct (decide (ρ = ρ')) as [-> | Hneq].
+        + inversion Htrans as [? Hbig]. destruct Hbig as (Hmap&Hleq&?&Hlim&?&?).
+          destruct (decide (ρ' ∈ live_roles _ δ')).
+          * rewrite Hsome /= in Hlim.
+            assert (Hlive: ρ' ∈ live_roles _ δ') by set_solver.
+            specialize (Hlim Hlive). lia.
+          * unfold fuel_decr in Hleq.
+            apply elem_of_dom_2 in Hmap. rewrite ls_same_doms in Hmap.
+            pose proof Hsome as Hsome'. apply elem_of_dom_2 in Hsome'.
+            specialize (Hleq ρ' ltac:(done) ltac:(done)).
+            assert(must_decrease ρ' (Some ρ') (trace_last atr) δ' (Some tid')) as Hmd; first by constructor 3.
+            specialize (Hleq Hmd). rewrite Hsome /= in Hleq.
+            apply elem_of_dom in Hmap as [? Heq]. rewrite Heq in Hleq.
+            pose proof (max_gmap_spec _ _ _ Heq). simpl in *. lia.
+        + inversion Htrans as [? Hbig]. destruct Hbig as (Hmap&?&Hleq'&?&Hnew&?).
+          destruct (decide (ρ ∈ dom $ ls_fuel (trace_last atr))) as [Hin|Hnotin].
+          * assert (Hok: oleq (ls_fuel δ' !! ρ) (ls_fuel (trace_last atr) !! ρ)).
+            { unfold fuel_must_not_incr in *.
+              assert (ρ ∈ dom $ ls_fuel (trace_last atr)) by SS.
+              specialize (Hleq' ρ ltac:(done) ltac:(congruence)) as [Hleq'|Hleq'] =>//. apply elem_of_dom_2 in Hsome. set_solver. }
+            rewrite Hsome in Hok. destruct (ls_fuel (trace_last atr) !! ρ) as [f'|] eqn:Heqn; last done.
+            pose proof (max_gmap_spec _ _ _ Heqn). simpl in *. lia.
+          * assert (Hok: oleq (ls_fuel δ' !! ρ) (Some (LM.(fuel_limit) δ'))).
+            { apply Hnew. apply elem_of_dom_2 in Hsome. set_solver. }
+            rewrite Hsome in Hok. simpl in Hok. lia.
+      - inversion Htrans as [? [? [Hleq [Hincl Heq]]]]. specialize (Hleq ρ).
+        assert (ρ ∈ dom $ ls_fuel (trace_last atr)) as Hin.
+        { apply elem_of_dom_2 in Hsome. set_solver. }
+        specialize (Hleq Hin ltac:(done)) as [Hleq|Hleq].
+        + rewrite Hsome in Hleq. destruct (ls_fuel (trace_last atr) !! ρ) as [f'|] eqn:Heqn. 
+          * pose proof (max_gmap_spec _ _ _ Heqn). simpl in *.
+            rewrite Heqn in Hleq.
+            lia.
+          * simpl in *. rewrite Heqn in Hleq. done.
+        + apply elem_of_dom_2 in Hsome. set_solver.
+      - inversion Htrans as [? [? [Hleq [Hnew Hfalse]]]]. done. }
+    apply elem_of_list_bind.
+    assert (Hmappingdom: dom δ'.(ls_mapping) = live_roles M δ' ∪ dom (ls_fuel δ')).
+    { rewrite -Hfueldom ls_same_doms //. }
+    exists (δ'.(ls_mapping) ↾ Hmappingdom); split; last first.
+    { eapply enum_gmap_range_bounded'_spec; split=>//.
+      intros ρ' tid' Hsome. unfold tids_smaller in *.
+      apply locales_of_list_from_locale_from. eauto. }
+    rewrite elem_of_list_singleton; f_equal.
+    - destruct δ'; simpl. f_equal; apply ProofIrrelevance.
+    - destruct ℓ; simpl; destruct oζ =>//; by inversion Hlbl.
+      Unshelve.
+      + intros ??. apply make_decision.
+      + intros. apply make_proof_irrel.
+      + done.
+      + done.
+  Qed.
+End finitary.
+
+Section finitary_simple.
+  Context `{M: FairModel}.
+  Context `{Λ: language}.
+  Context `{LM: LiveModel Λ M}.
+  Context `{EqDecision M}.
+  Context `{EqDecision (locale Λ)}.
+
+  Context `{HPI0: forall s x, ProofIrrel ((let '(s', ℓ) := x in M.(fmtrans) s ℓ s'): Prop) }.
+
+  Variable model_finitary: forall s1, Finite { '(s2, ℓ) | M.(fmtrans) s1 ℓ s2 }.
+
+  Definition enum_inner_simple (s1: M): list (M * option M.(fmrole)) :=
+    map proj1_sig (@enum _ _ (model_finitary s1)).
+
+  Lemma enum_inner_spec_simple (s1 s2: M) ℓ:
+    M.(fmtrans) s1 ℓ s2 -> (s2, ℓ) ∈ enum_inner_simple s1.
+  Proof.
+    intros H. unfold enum_inner. rewrite elem_of_list_fmap.
+    exists (exist _ (s2, ℓ) H). split =>//. apply elem_of_enum.
+  Qed.
+
+  Program Definition enumerate_next_simple (δ1: LM) (oζ : olocale Λ) (c': cfg Λ):
+    list (LM * @mlabel LM) :=
+    '(s2, ℓ) ← (δ1.(ls_under), None) :: enum_inner_simple δ1.(ls_under);
+    d ← enumerate_dom_gsets' (dom δ1.(ls_fuel) ∪ live_roles _ s2);
+    fs ← enum_gmap_bounded' (live_roles _ s2 ∪ d) (max_gmap δ1.(ls_fuel) `max` LM.(fuel_limit) s2);
+    ms ← enum_gmap_range_bounded' (live_roles _ s2 ∪ d) (locales_of_list c'.1);
+    let ℓ' := match ℓ with
+              | None => match oζ with
+                         Some ζ => Silent_step ζ
+                       | None => Config_step
+                       end
+              | Some ℓ => match oζ with
+                         | None => Config_step
+                         | Some ζ => Take_step ℓ ζ
+                         end
+              end in
+    mret ({| ls_under := s2;
+             ls_fuel := `fs;
+             (* ls_fuel_dom := proj2_sig fs; *) (* TODO: why this does not work?*)
+             ls_mapping := `ms ;
+          |}, ℓ').
+  Next Obligation.
+    intros ??????????. destruct fs as [? Heq]. rewrite /= Heq //. set_solver.
+  Qed.
+  Next Obligation.
+    intros ??????????. destruct fs as [? Heq]. destruct ms as [? Heq'].
+    rewrite /= Heq //.
+  Qed.
+
+  (* TODO: Derive this from the stronger version *)
+  Lemma valid_state_evolution_finitary_fairness_simple (φ: execution_trace Λ -> auxiliary_trace LM -> Prop) :
     rel_finitary (valid_lift_fairness φ).
   Proof.
     intros extr auxtr [e' σ'] oζ.
     eapply finite_smaller_card_nat.
-    eapply (in_list_finite (enumerate_next (trace_last auxtr) oζ (e',σ'))).
+    eapply (in_list_finite (enumerate_next_simple (trace_last auxtr) oζ (e',σ'))).
     intros [δ2 ℓ] [[Hlab [Htrans Hsmall]] ?].
     unfold enumerate_next. apply elem_of_list_bind.
     exists (δ2.(ls_under), match ℓ with Take_step l _ => Some l | _ => None end).
     split; last first.
     { destruct ℓ as [ρ tid' | |].
-      - inversion Htrans as [Htrans']. apply elem_of_cons; right. by apply enum_inner_spec.
+      - inversion Htrans as [Htrans']. apply elem_of_cons; right. by apply enum_inner_spec_simple.
       - apply elem_of_cons; left. f_equal. inversion Htrans as (?&?&?&?&?); done.
-      - apply elem_of_cons; right. inversion Htrans as (?&?). by apply enum_inner_spec. }
+      - apply elem_of_cons; right. inversion Htrans as (?&?). by apply enum_inner_spec_simple. }
     apply elem_of_list_bind. eexists (dom $ δ2.(ls_fuel)). split; last first.
     { apply enumerate_dom_gsets'_spec. destruct ℓ as [ρ tid' | |].
       - inversion Htrans as (?&?&?&?&?&?&?). intros ρ' Hin. destruct (decide (ρ' ∈ live_roles _ δ2)); first set_solver.
@@ -146,4 +319,44 @@ Section finitary.
       + done.
       + done.
   Qed.
-End finitary.
+End finitary_simple.
+
+Definition live_rel `(LM: LiveModel Λ M) `{EqDecision (locale Λ)}
+           (ex : execution_trace Λ) (aux : auxiliary_trace LM) :=
+  live_tids (M := M) (trace_last ex) (trace_last aux).
+
+Definition sim_rel `(LM: LiveModel Λ M) `{EqDecision (locale Λ)}
+           (ex : execution_trace Λ) (aux : auxiliary_trace LM) :=
+  valid_state_evolution_fairness ex aux ∧ live_rel LM ex aux.
+
+Definition sim_rel_with_user `(LM: LiveModel Λ M) `{EqDecision (locale Λ)}
+           (ξ : execution_trace Λ -> finite_trace M (option (fmrole M)) -> Prop)
+  (ex : execution_trace Λ) (aux : auxiliary_trace LM) :=
+  sim_rel LM ex aux ∧ ξ ex (map_underlying_trace aux).
+
+(* TODO: Maybe redefine [sim_rel_with_user] in terms of [valid_lift_fairness] *)
+Lemma valid_lift_fairness_sim_rel_with_user `{LM:LiveModel Λ Mdl}
+      `{EqDecision (locale Λ)}
+      (ξ : execution_trace Λ → finite_trace Mdl (option $ fmrole Mdl) →
+           Prop) extr atr :
+  valid_lift_fairness
+    (λ extr auxtr, ξ extr (map_underlying_trace (LM:=LM) auxtr) ∧
+                   live_rel LM extr auxtr) extr atr ↔
+  sim_rel_with_user LM ξ extr atr.
+Proof. split; [by intros [Hvalid [Hlive Hξ]]|by intros [[Hvalid Hlive] Hξ]]. Qed.
+
+Lemma rel_finitary_sim_rel_with_user_ξ `{LM:LiveModel Λ Mdl}
+      `{EqDecision (locale Λ)} ξ :
+  rel_finitary ξ → rel_finitary (sim_rel_with_user LM ξ).
+Proof.
+  intros Hrel.
+  eapply rel_finitary_impl.
+  { intros ex aux. by eapply valid_lift_fairness_sim_rel_with_user.
+    (* TODO: Figure out if these typeclass subgoals should be resolved locally *)
+    Unshelve.
+    - intros ??. apply make_decision.
+    - intros ??. apply make_decision. }
+  by eapply valid_state_evolution_finitary_fairness.
+  Unshelve.
+  - intros ??. apply make_proof_irrel.
+Qed.
