fairness/examples/choose_nat/choose_nat.v
@@ -1,0 +1,387 @@
+From stdpp Require Import finite decidable.
+From iris.prelude Require Import options.
+From iris.algebra Require Import excl_auth.
+From iris.bi Require Import bi.
+From iris.base_logic.lib Require Import invariants.
+From iris.proofmode Require Import tactics.
+From trillium.prelude Require Export finitary quantifiers sigma classical_instances.
+From trillium.fairness Require Import fairness fair_termination fairness_finiteness.
+From trillium.program_logic Require Export weakestpre.
+From trillium.fairness.heap_lang Require Export lang lifting tactics proofmode.
+From trillium.fairness.heap_lang Require Import notation.
+
+Import derived_laws_later.bi.
+
+Set Default Proof Using "Type".
+
+(** The program verify liveness for *)
+(** Recursion is "off by one" to allow immediate termination after storing 0 *)
+Definition decr_loop_prog (l : loc) : val :=
+  rec: "go" <> :=
+    let: "x" := !#l in
+    if: "x" = #1 then #l <- ("x" - #1)
+    else #l <- ("x" - #1);; "go" #().
+Definition choose_nat_prog (l : loc) : val :=
+  λ: <>,
+     #l <- (ChooseNat + #1);;
+     decr_loop_prog l #().
+
+(** The model state *)
+Inductive CN := Start | N (n : nat).
+
+(** A mapping of model state to "program state" *)
+Definition CN_Z (cn : CN) : Z :=
+  match cn with
+  | Start => -1
+  | N n => n
+  end.
+
+#[global] Instance CN_eqdec: EqDecision CN.
+Proof. solve_decision. Qed.
+
+#[global] Instance CN_inhabited: Inhabited CN.
+Proof. exact (populate Start). Qed.
+
+Inductive cntrans : CN → option unit → CN -> Prop :=
+| start_trans n : cntrans Start (Some ()) (N n)
+| decr_trans n : cntrans (N $ S n) (Some ()) (N n).
+
+(* Free construction of the active labels on each state by [cntrans] *)
+Definition cn_live_roles (cn : CN) : gset unit :=
+  match cn with N 0 => ∅ | _ => {[ () ]} end.
+
+Lemma cn_live_spec_holds s ρ s' : cntrans s (Some ρ) s' -> ρ ∈ cn_live_roles s.
+Proof. destruct s; [set_solver|]. destruct n; [|set_solver]. inversion 1. Qed.
+
+Definition cn_fair_model : FairModel.
+Proof.
+  refine({|
+            fmstate := CN;
+            fmrole := unit;
+            fmtrans := cntrans;
+            live_roles := cn_live_roles;
+            fm_live_spec := cn_live_spec_holds;
+          |}).
+Defined.
+
+(** Show that the model is fairly terminating *)
+
+Inductive cn_order : CN → CN → Prop :=
+  | cn_order_Start cn : cn_order cn Start
+  | cn_order_N (n1 n2 : nat) : n1 ≤ n2 → cn_order (N n1) (N n2).
+
+Local Instance the_order_po: PartialOrder cn_order.
+Proof.
+  split.
+  - split.
+    + by intros []; constructor.
+    + intros [] [] [] Hc12 Hc23; try constructor.
+      * inversion Hc23.
+      * inversion Hc12.
+      * inversion Hc23.
+      * inversion Hc12. inversion Hc23. simplify_eq. lia.
+  - intros [] []; inversion 1; simplify_eq; try eauto; try inversion 1.
+    simplify_eq. f_equal. lia.
+Qed.
+
+Definition cn_decreasing_role (s : fmstate cn_fair_model) : unit :=
+  match s with | _ => () end.
+
+#[local] Program Instance cn_model_terminates :
+  FairTerminatingModel cn_fair_model :=
+  {|
+    ftm_leq := cn_order;
+    ftm_decreasing_role := cn_decreasing_role;
+  |}.
+Next Obligation.
+  assert (∀ n, Acc (strict cn_order) (N n)).
+  { intros n.
+    induction n as [n IHn] using lt_wf_ind.
+    constructor. intros cn [Hcn1 Hcn2].
+    inversion Hcn1 as [|n1 n2]; simplify_eq.
+    destruct (decide (n = n1)) as [->|Hneq]; [done|].
+    apply IHn. lia. }
+  constructor. intros [] [Hc1 Hc2]; [|done].
+  inversion Hc1; simplify_eq. done.
+Qed.
+Next Obligation.
+  intros cn [ρ' [cn' Htrans]].
+  split.
+  - rewrite /cn_decreasing_role. simpl. rewrite /cn_live_roles.
+    destruct cn; [set_solver|].
+    destruct n; [inversion Htrans|set_solver].
+  - intros cn'' Htrans'.
+    destruct cn.
+    + split; [constructor|].
+      intros Hrel. inversion Hrel; simplify_eq. inversion Htrans'.
+    + split.
+      * destruct cn''.
+        -- inversion Htrans'.
+        -- inversion Htrans'; simplify_eq. constructor. lia.
+      * intros Hrel.
+        inversion Htrans'; simplify_eq.
+        inversion Hrel; simplify_eq.
+        lia.
+Qed.
+Next Obligation. done. Qed.
+Next Obligation.
+  intros cn1 ρ cn2 Htrans.
+  destruct cn1.
+  - inversion Htrans; simplify_eq. constructor.
+  - inversion Htrans; simplify_eq. constructor. lia.
+Qed.
+
+Definition cn_model : LiveModel heap_lang cn_fair_model :=
+  {| fuel_limit _ := 40%nat |}.
+
+(** Determine additional restriction on relation to obtain finite branching *)
+Definition ξ_cn (l:loc) (extr : execution_trace heap_lang)
+           (auxtr : finite_trace cn_fair_model (option unit)) :=
+  ∃ (cn:CN), (trace_last extr).2.(heap) !!! l = #(CN_Z cn) ∧
+             (trace_last auxtr) = cn.
+
+(** Verify that the program refines the model *)
+
+(* Set up necessary RA constructions *)
+Class choose_natG Σ := ChooseNatG { choose_nat_G :> inG Σ (excl_authR ZO) }.
+
+Definition choose_natΣ : gFunctors :=
+  #[ heapΣ cn_fair_model; GFunctor (excl_authR ZO) ].
+
+Global Instance subG_choosenatΣ {Σ} : subG choose_natΣ Σ → choose_natG Σ.
+Proof. solve_inG. Qed.
+
+Definition Ns := nroot .@ "choose_nat".
+
+Section proof.
+  Context `{!heapGS Σ cn_fair_model cn_model, choose_natG Σ}.
+
+  (** Determine invariant so we can eventually derive ξ_cn from it *)
+  Definition choose_nat_inv_inner (γ : gname) (l:loc) : iProp Σ :=
+    ∃ (cn:CN), frag_model_is cn ∗ l ↦ #(CN_Z cn) ∗ own γ (●E (CN_Z cn)).
+
+  Definition choose_nat_inv (γ : gname) (l:loc) :=
+    inv Ns (choose_nat_inv_inner γ l).
+
+  Lemma decr_loop_spec γ tid l (n:nat) (f:nat) :
+    7 ≤ f → f ≤ 38 →
+    choose_nat_inv γ l -∗
+    {{{ has_fuel tid () f ∗ frag_free_roles_are ∅ ∗
+        own γ (◯E (Z.of_nat (S n))) }}}
+      decr_loop_prog l #() @ tid ; ⊤
+    {{{ RET #(); tid ↦M ∅ }}}.
+  Proof.
+    iIntros (Hle1 Hle2) "#IH".
+    iIntros "!>" (Φ) "(Hf & Hr & Hm) HΦ".
+    iInduction n as [|n] "IHn".
+    { wp_lam.
+      (* Load - with invariant *)
+      wp_bind (Load _).
+      iApply wp_atomic.
+      iInv Ns as ">HI" "Hclose".
+      iDestruct "HI" as (cn) "(Hs & Hl & Hcn)".
+      iDestruct (own_valid_2 with "Hcn Hm") as %Hvalid%excl_auth_agree_L.
+      iModIntro.
+      wp_load.
+      iModIntro.
+      iMod ("Hclose" with "[Hs Hl Hcn]") as "_"; [ iExists _; iFrame | ].
+      iModIntro.
+      rewrite Hvalid. clear cn Hvalid.
+      (* Store - with invariant *)
+      wp_pures.
+      replace (Z.of_nat 1 - 1)%Z with 0%Z by lia.
+      wp_bind (Store _ _).
+      iApply wp_atomic.
+      iInv Ns as ">HI" "Hclose".
+      iDestruct "HI" as (cn) "(Hs & Hl & Hcn)".
+      iDestruct (own_valid_2 with "Hcn Hm") as %Hvalid%excl_auth_agree_L.
+      iModIntro.
+      assert (cn = N 1) as ->.
+      { destruct cn; inversion Hvalid. by simplify_eq. }
+      (* Update the model state to maintain program correspondence *)
+      iApply (wp_store_step_singlerole _ _ (():fmrole cn_fair_model) (f - 7) (f-3)
+               with "[$Hl $Hs $Hr Hf]").
+      { simpl. lia. }
+      { constructor. }
+      { set_solver. }
+      { replace (f - 1 - 1 - 1 - 1 - 1 - 1 - 1)%nat with (f - 7)%nat by lia.
+        by rewrite has_fuel_fuels. }
+      iIntros "!> (Hl & Hs & Hr & Hf)".
+      iMod (own_update_2 _ _ _ with "Hcn Hm") as "[Hcn Hm]".
+      { apply (excl_auth_update _ _ 0%Z). }
+      iMod ("Hclose" with "[Hs Hl Hcn]") as "_".
+      { iExists (N 0). iFrame. }
+      iModIntro.
+      simpl.
+      destruct (decide (() ∈ ∅)); [set_solver|].
+      by iApply "HΦ". }
+    wp_lam.
+    (* Load - with invariant *)
+    wp_bind (Load _).
+    iApply wp_atomic.
+    iInv Ns as ">HI" "Hclose".
+    iModIntro.
+    iDestruct "HI" as (cn) "(Hs & Hl & Hcn)".
+    wp_load.
+    iDestruct (own_valid_2 with "Hcn Hm") as %Hvalid%excl_auth_agree_L.
+    iModIntro. iMod ("Hclose" with "[Hs Hl Hcn]") as "_".
+    { iExists _. iFrame. }
+    iModIntro.
+    rewrite Hvalid. clear cn Hvalid.
+    wp_pures.
+    case_bool_decide as Heq; [inversion Heq; lia|clear Heq].
+    wp_pures.
+    replace (Z.of_nat (S (S n))  - 1)%Z with (Z.of_nat (S n)) %Z by lia.
+    (* Store - with invariant *)
+    wp_bind (Store _ _).
+    iApply wp_atomic.
+    iInv Ns as ">HI" "Hclose".
+    iModIntro.
+    iDestruct "HI" as (cn) "(Hs & Hl & Hcn)".
+    iDestruct (own_valid_2 with "Hcn Hm") as %Hvalid%excl_auth_agree_L.
+    assert (cn = N (S (S n))) as ->.
+    { destruct cn; inversion Hvalid. by simplify_eq. }
+    (* Update the model state to maintain program correspondence *)
+    iApply (wp_store_step_singlerole _ _ (():fmrole cn_fair_model) (f - 7)
+                                     (f+2) with "[$Hl $Hs $Hr Hf]").
+    { simpl. lia. }
+    { constructor. }
+    { set_solver. }
+    { replace (f - 1 - 1 - 1 - 1 - 1 - 1 - 1)%nat with (f - 7)%nat by lia.
+      rewrite has_fuel_fuels. done. }
+    iIntros "!> (Hl & Hs & Hr & Hf)".
+    iMod (own_update_2 _ _ _ with "Hcn Hm") as "[Hcn Hm]".
+    { apply (excl_auth_update _ _ (Z.of_nat (S n))%Z). }
+    iMod ("Hclose" with "[Hs Hl Hcn]") as "_".
+    { iExists (N (S n)). iFrame. }
+    iModIntro.
+    simpl. destruct (decide (() ∈ {[()]})); [|set_solver].
+    wp_pures.
+    replace (f + 2 - 1 - 1)%nat with f by lia.
+    by iApply ("IHn" with "Hf Hr Hm").
+  Qed.
+
+  Lemma choose_nat_spec γ l tid (f:nat) :
+    12 ≤ f → f ≤ 40 →
+    choose_nat_inv γ l -∗
+    {{{ has_fuel tid () f ∗ frag_free_roles_are ∅ ∗ own γ (◯E (-1)%Z) }}}
+      choose_nat_prog l #() @ tid
+    {{{ RET #(); tid ↦M ∅ }}}.
+  Proof.
+    iIntros (Hle1 Hle2) "#IH".
+    iIntros "!>" (Φ) "(Hf & Hr & Hm) HΦ".
+    wp_lam.
+    wp_bind ChooseNat.
+    iApply (wp_choose_nat_nostep _ _ _ {[() := (f - 2)%nat]} with "[Hf]").
+    { set_solver. }
+    { rewrite -has_fuel_fuels_S has_fuel_fuels.
+      replace (S (f - 2))%nat with (f - 1)%nat by lia. done. }
+    iIntros "!>" (n) "Hf".
+    wp_pures.
+    (* Store - with invariant *)
+    wp_bind (Store _ _).
+    iApply wp_atomic.
+    iInv Ns as ">HI" "Hclose".
+    iModIntro.
+    iDestruct "HI" as (cn) "(Hs & Hl & Hcn)".
+    iDestruct (own_valid_2 with "Hcn Hm") as %Hvalid%excl_auth_agree_L.
+    assert (cn = Start) as ->.
+    { destruct cn; inversion Hvalid; [done|]. lia. }
+    (* Update the model state to maintain program correspondence *)
+    iApply (wp_store_step_singlerole _ _ (():fmrole cn_fair_model)
+                                     (f - 3) (f-2) _ _ (N (S n))
+             with "[$Hl $Hs $Hr Hf]").
+    { simpl. lia. }
+    { constructor. }
+    { set_solver. }
+    { replace (f - 2 - 1)%nat with (f - 3)%nat by lia.
+      rewrite has_fuel_fuels. done. }
+    iIntros "!> (Hl & Hs & Hr & Hf)".
+    iMod (own_update_2 _ _ _ with "Hcn Hm") as "[Hcn Hm]".
+    { apply (excl_auth_update _ _ (Z.of_nat (S n))%Z). }
+    iMod ("Hclose" with "[Hs Hl Hcn]") as "_".
+    { replace (Z.of_nat n + 1)%Z with (Z.of_nat (S n)) by lia.
+      iExists (N (S n)). iFrame. }
+    iModIntro.
+    simpl. destruct (decide (() ∈ {[()]})); [|set_solver].
+    wp_pures.
+    rewrite -has_fuel_fuels.
+    by iApply (decr_loop_spec with "IH [$Hm $Hr $Hf]"); [lia|lia|].
+  Qed.
+
+End proof.
+
+(** Construct inverse mapping of program state to model state,
+    to compute finite relation *)
+Definition Z_CN (v : val) : CN :=
+  match v with
+  | LitV (LitInt z) =>
+      match z with
+      | Z0 => N 0
+      | Zpos p => N (Pos.to_nat p)
+      | Zneg _ => Start         (* Error case when z < -1 *)
+      end
+  | _ => Start                  (* Error case *)
+  end.
+
+Lemma Z_CN_CN_Z cn : Z_CN #(CN_Z cn) = cn.
+Proof. destruct cn; [done|]; destruct n; [done|]=> /=; f_equal; lia. Qed.
+
+(** Derive that program is related to model by
+    [sim_rel_with_user cn_model (ξ_cn l) using Trillium adequacy *)
+Lemma choose_nat_sim l :
+  continued_simulation
+    (sim_rel_with_user cn_model (ξ_cn l))
+    (trace_singleton ([choose_nat_prog l #()],
+                        {| heap := {[l:=#-1]};
+                           used_proph_id := ∅ |}))
+    (trace_singleton (initial_ls (LM := cn_model) Start 0%nat)).
+Proof.
+  assert (heapGpreS choose_natΣ cn_fair_model cn_model) as HPreG.
+  { apply _. }
+  eapply (strong_simulation_adequacy (Mdl := cn_fair_model)
+            choose_natΣ NotStuck _ _ _ ∅); [|set_solver|].
+  { clear.
+    apply rel_finitary_sim_rel_with_user_ξ.
+    intros extr atr c' oζ.
+    eapply finite_smaller_card_nat=> /=.
+    eapply (in_list_finite [(Z_CN (heap c'.2 !!! l), None);
+                            (Z_CN (heap c'.2 !!! l), Some ())]).
+    (* TODO: Figure out why this does not unify with typeclass *)
+    Unshelve. 2: intros x; apply make_proof_irrel.
+    intros [cn o] [cn' [Hextr Hatr]].
+    rewrite Hextr Z_CN_CN_Z -Hatr. destruct o; [destruct u|]; set_solver. }
+  iIntros (?) "!> Hσ Hs Hr Hf".
+  iMod (own_alloc) as (γ) "He"; [apply (excl_auth_valid (-1)%Z)|].
+  iDestruct "He" as "[He● He○]".
+  iMod (inv_alloc Ns ⊤ (choose_nat_inv_inner γ l) with "[He● Hσ Hs]") as "#IH".
+  { iIntros "!>". iExists _. iFrame. by rewrite big_sepM_singleton. }
+  iModIntro.
+  iSplitL.
+  { iApply (choose_nat_spec _ _ _ 40 with "IH [Hr Hf He○]");
+      [lia|lia| |by eauto]=> /=.
+    replace (∅ ∖ {[()]}) with (∅:gset unit) by set_solver.
+    rewrite has_fuel_fuels gset_to_gmap_set_to_map. iFrame. }
+  iIntros (ex atr c Hvalid Hex Hatr Hends Hξ Hstuck) "Hσ".
+  iInv Ns as ">H".
+  iDestruct "H" as (cn) "(Hf & Hl & H●)".
+  iDestruct "Hσ" as (Hvalid') "[Hσ Hs]".
+  iDestruct (gen_heap_valid with "Hσ Hl") as %Hlookup%lookup_total_correct.
+  iDestruct (model_agree' with "Hs Hf") as %Hlast.
+  iModIntro. iSplitL; [by iExists _; iFrame|].
+  iApply fupd_mask_intro; [set_solver|]. iIntros "_".
+  iPureIntro. exists cn.
+  split; [done|].
+  subst. by destruct atr.
+Qed.
+
+Theorem choose_nat_terminates l extr :
+  trfirst extr = ([choose_nat_prog l #()],
+                    {| heap := {[l:=#-1]};
+                      used_proph_id := ∅ |}) →
+  extrace_fairly_terminating extr.
+Proof.
+  intros Hexfirst.
+  eapply heap_lang_continued_simulation_fair_termination; eauto.
+  rewrite Hexfirst. eapply choose_nat_sim.
+Qed.
